Generating free algebras and equational theories, for no particular reason.

garbage/FieldThyGen.hs
@@ -1,0 +1,172 @@
+module Main where
+
+import Control.Applicative
+import Control.Monad
+import Data.Char
+import Data.Foldable
+import Data.Map
+import Data.Ratio
+import Numeric
+
+subscribe :: Int -> Char
+subscribe i = chr (ord '\x2080' + i)
+
+data Nots = Arith
+  deriving (Eq, Ord, Show)
+
+data Expr = Var Int | Add Expr Expr | Zero | Neg Expr |
+  Mul Expr Expr | One | Recip Expr
+  deriving (Eq, Ord, Show)
+
+showsNots :: Nots -> Expr -> ShowS
+showsNots _ Var {} = showString "x"
+showsNots Arith Add {} = showString " + "
+showsNots Arith Zero {} = showString "0"
+showsNots Arith Neg {} = showString "- "
+showsNots Arith Mul {} = showString " \xd7 "
+showsNots Arith One {} = showString "1"
+showsNots Arith Recip {} = showString "/ "
+
+showsPrecExpr :: Int -> Nots -> Expr -> ShowS
+showsPrecExpr _ cs e @ (Var i) = showsNots cs e . showChar (subscribe i)
+showsPrecExpr n cs e @ (Add x y) = showParen (n > 6)
+  (showsPrecExpr 7 cs x . showsNots cs e . showsPrecExpr 7 cs y)
+showsPrecExpr _ cs e @ Zero = showsNots cs e
+showsPrecExpr n cs e @ (Neg x) = showParen (n > 7)
+  (showsNots cs e . showsPrecExpr 8 cs x)
+showsPrecExpr n cs e @ (Mul x y) = showParen (n > 8)
+  (showsPrecExpr 9 cs x . showsNots cs e . showsPrecExpr 9 cs y)
+showsPrecExpr _ cs e @ One = showsNots cs e
+showsPrecExpr n cs e @ (Recip x) = showParen (n > 9)
+  (showsNots cs e . showsPrecExpr 10 cs x)
+
+showsExpr :: Nots -> Expr -> ShowS
+showsExpr = showsPrecExpr 0
+
+showExpr :: Nots -> Expr -> String
+showExpr cs e = showsExpr cs e mempty
+
+manglesExpr :: Expr -> ShowS
+manglesExpr = let
+  f _ e @ (Var i) = showChar 'v' . showInt i
+  f n e @ (Add x y) = (\ k ->
+    if n > 6 then showChar 'o' . k . showChar 'c' else k)
+    (f 7 x . showChar 'a' . f 7 y)
+  f _ e @ Zero = showChar 'z'
+  f n e @ (Neg x) = (\ k ->
+    if n > 7 then showChar 'o' . k . showChar 'c' else k)
+    (showChar 'n' . f 8 x)
+  f n e @ (Mul x y) = (\ k ->
+    if n > 8 then showChar 'o' . k . showChar 'c' else k)
+    (f 9 x . showChar 'm' . f 9 y)
+  f _ e @ One = showChar 'w'
+  f n e @ (Recip x) = (\ k ->
+    if n > 9 then showChar 'o' . k . showChar 'c' else k)
+    (showChar 'r' . f 10 x) in
+  f 0
+
+mangleExpr :: Expr -> String
+mangleExpr e = manglesExpr e mempty
+
+genExpr :: Int -> [Expr]
+genExpr n = case n of
+  0 -> Zero : One : [Var i | i <- [0 .. 1]]
+  i -> genExpr 0 ++ do
+    x <- genExpr (pred n)
+    Neg x : Recip x : do
+      y <- genExpr (pred n)
+      [Add x y, Mul x y]
+
+evalExpr :: (Eq a, Fractional a) => (Int -> a) -> Expr -> a
+evalExpr f e = case e of
+  Var i -> f i
+  Add x y -> evalExpr f x + evalExpr f y
+  Zero -> 0
+  Neg x -> negate (evalExpr f x)
+  Mul x y -> evalExpr f x * evalExpr f y
+  One -> 1
+  Recip x -> case evalExpr f x of
+    0 -> 0
+    y -> recip y
+
+occurs :: Expr -> Map Int Int
+occurs e = case e of
+  Var i -> singleton i 1
+  Add x y -> unionWith (+) (occurs x) (occurs y)
+  Zero -> mempty
+  Neg x -> occurs x
+  Mul x y -> unionWith (+) (occurs x) (occurs y)
+  One -> mempty
+  Recip x -> occurs x
+
+isAffine :: Expr -> Bool
+isAffine = all (== 1) . occurs
+
+occursPoint :: Expr -> Map Bool Int
+occursPoint e = case e of
+  Var i -> mempty
+  Add x y -> unionWith (+) (occursPoint x) (occursPoint y)
+  Zero -> singleton (toEnum 0) 1
+  Neg x -> occursPoint x
+  Mul x y -> unionWith (+) (occursPoint x) (occursPoint y)
+  One -> singleton (toEnum 1) 1
+  Recip x -> occursPoint x
+
+isAffinePoint :: Expr -> Bool
+isAffinePoint = all (== 1) . occursPoint
+
+constrs :: Expr -> Int
+constrs e = case e of
+  Var i -> 1
+  Add x y -> 1 + constrs x + constrs y
+  Zero -> 1
+  Neg x -> 1 + constrs x
+  Mul x y -> 1 + constrs x + constrs y
+  One -> 1
+  Recip x -> 1 + constrs x
+
+exprs :: Int -> IO ()
+exprs n = traverse_ (putStrLn . showExpr Arith) (genExpr n)
+
+data Eqn = Eqn Expr Expr
+  deriving (Eq, Ord, Show)
+
+showsEqn :: Nots -> Eqn -> ShowS
+showsEqn cs (Eqn x y) = showsExpr cs x . showString " = " . showsExpr cs y
+
+showEqn :: Nots -> Eqn -> String
+showEqn cs e = showsEqn cs e mempty
+
+manglesEqn :: Eqn -> ShowS
+manglesEqn (Eqn x y) = manglesExpr x . showChar 'e' . manglesExpr y
+
+mangleEqn :: Eqn -> String
+mangleEqn e = manglesEqn e mempty
+
+eqns :: Int -> IO ()
+eqns n = let
+  f :: Rational -> Rational -> Int -> Rational
+  f a b = (a +) . (b *) . fromIntegral
+  g :: Rational -> Rational -> Expr -> Rational
+  g a b = evalExpr (f a b)
+  xs = do
+    x <- genExpr n
+    y <- genExpr n
+    -- Only irreflexive asymmetric equations are of interest...
+    guard (x < y)
+    -- ...as long as they are affine in all the variables...
+    guard (isAffinePoint x && isAffinePoint y)
+    guard (constrs x < 6 && constrs y < 6)
+    -- ...if they are satisfied in a linear subspace
+    -- (that is, they are not obviously false).
+    guard (and [g a b x == g a b y | a <- [7, 11, 13], b <- [2, 3, 5]])
+    pure (Eqn x y) in
+  traverse_ (putStrLn . showEqn Arith) xs
+
+main :: IO ()
+main = do
+  putStrLn "Once upon a time in an algebra..."
+  exprs 1
+  putStrLn "...until they came across an equational theory..."
+  eqns 1
+  putStrLn "...the end."
