bird/Is/TwoSortedly/LeftUnital.v
@@ -3,6 +3,6 @@ From Maniunfold.Has Require Export
 From Maniunfold.ShouldHave Require Import
   EquivalenceRelationNotations AdditiveNotations.
 
-Class IsLUnl2 {A B : Type} {has_eq_rel : HasEqRel B}
+Class IsTwoLUnl {A B : Type} {has_eq_rel : HasEqRel B}
   (has_l_un : HasLUn A) (has_l_act : HasLAct A B) : Prop :=
-  l_unl_2 : forall x : B, L0 L+ x == x.
+  two_l_unl : forall x : B, L0 L+ x == x.
