bird/Is/TwoSortedly/RightUnital.v
@@ -3,6 +3,6 @@ From Maniunfold.Has Require Export
 From Maniunfold.ShouldHave Require Import
   EquivalenceRelationNotations AdditiveNotations.
 
-Class IsRUnl2 {A B : Type} {has_eq_rel : HasEqRel B}
+Class IsTwoRUnl {A B : Type} {has_eq_rel : HasEqRel B}
   (has_r_un : HasRUn A) (has_r_act : HasRAct A B) : Prop :=
-  r_unl_2 : forall x : B, x R+ R0 == x.
+  two_r_unl : forall x : B, x R+ R0 == x.
