bird/Is/TwoSortedly/Unital.v
@@ -3,9 +3,9 @@ From Maniunfold.Has Require Export
 From Maniunfold.Is Require Export
   LeftUnital RightUnital.
 
-Class IsUnl2 {A B : Type} {has_eq_rel : HasEqRel B}
+Class IsTwoUnl {A B : Type} {has_eq_rel : HasEqRel B}
   (has_l_un : HasLUn A) (has_r_un : HasRUn A)
   (has_l_act : HasLAct A B) (has_r_act : HasRAct A B) : Prop := {
-  l_un_l_act_is_l_unl_2 :> IsLUnl2 l_un l_act;
-  r_un_r_act_is_r_unl_2 :> IsRUnl2 r_un r_act;
+  l_un_l_act_is_two_l_unl_ :> IsTwoLUnl l_un l_act;
+  r_un_r_act_is_two_r_unl_ :> IsTwoRUnl r_un r_act;
 }.
