bird/Is/OneSortedly/BinaryCommutative.v
@@ -7,18 +7,6 @@ From Maniunfold.Is Require Export
 
 Class IsBinComm {A : Type} {has_eq_rel : HasEqRel A}
   (has_un_op : HasUnOp A) (has_bin_op : HasBinOp A) : Prop := {
-  bin_op_un_op_is_l_bin_comm :> IsLBinComm un_op bin_op;
-  bin_op_un_op_is_r_bin_comm :> IsRBinComm un_op bin_op;
+  un_op_bin_op_is_l_bin_comm :> IsLBinComm un_op bin_op;
+  un_op_bin_op_is_r_bin_comm :> IsRBinComm un_op bin_op;
 }.
-
-Section Context.
-
-Context {A : Type} `{is_bin_comm : IsBinComm A}.
-
-Global Instance bin_op_un_op_is_ext_bin_comm : IsExtBinComm un_op bin_op.
-Proof.
-  constructor.
-  - destruct is_bin_comm; typeclasses eauto.
-  - destruct is_bin_comm; typeclasses eauto. Qed.
-
-End Context.
