bird/Is/OneSortedly/Invertible.v
@@ -1,7 +1,7 @@
 From Maniunfold.Has Require Export
   EquivalenceRelation BinaryOperation Unit UnaryOperation.
 From Maniunfold.Is Require Export
-  LeftInvertible RightInvertible ExternallyInvertible.
+  LeftInvertible RightInvertible.
 
 Class IsInv {A : Type} {has_eq_rel : HasEqRel A}
   (has_bin_op : HasBinOp A) (has_un : HasUn A)
@@ -9,16 +9,3 @@ Class IsInv {A : Type} {has_eq_rel : HasEqRel A}
   bin_op_un_un_op_is_l_inv :> IsLInv bin_op un un_op;
   bin_op_un_un_op_is_r_inv :> IsRInv bin_op un un_op;
 }.
-
-Section Context.
-
-Context {A : Type} `{is_inv : IsInv A}.
-
-Global Instance bin_op_un_un_op_is_ext_inv :
-  IsExtInv un un un_op un_op bin_op bin_op.
-Proof.
-  constructor.
-  - destruct is_inv; typeclasses eauto.
-  - destruct is_inv; typeclasses eauto. Qed.
-
-End Context.
