bird/Is/OneSortedly/LeftInvertible.v
@@ -1,7 +1,5 @@
 From Maniunfold.Has Require Export
   EquivalenceRelation BinaryOperation Unit UnaryOperation.
-From Maniunfold.Is Require Export
-  LeftExternallyInvertible.
 From Maniunfold.ShouldHave Require Import
   EquivalenceRelationNotations AdditiveNotations.
 
@@ -9,12 +7,3 @@ Class IsLInv {A : Type} {has_eq_rel : HasEqRel A}
   (has_bin_op : HasBinOp A) (has_un : HasUn A)
   (has_un_op : HasUnOp A) : Prop :=
   l_inv : forall x : A, - x + x == 0.
-
-Section Context.
-
-Context {A : Type} `{is_l_inv : IsLInv A}.
-
-Global Instance bin_op_un_un_op_is_l_ext_inv : IsLExtInv un un_op bin_op.
-Proof. intros x. apply l_inv. Qed.
-
-End Context.
