bird/Is/OneSortedly/RightInvertible.v
@@ -1,7 +1,5 @@
 From Maniunfold.Has Require Export
   EquivalenceRelation BinaryOperation Unit UnaryOperation.
-From Maniunfold.Is Require Export
-  RightExternallyInvertible.
 From Maniunfold.ShouldHave Require Import
   EquivalenceRelationNotations AdditiveNotations.
 
@@ -9,12 +7,3 @@ Class IsRInv {A : Type} {has_eq_rel : HasEqRel A}
   (has_bin_op : HasBinOp A) (has_un : HasUn A)
   (has_un_op : HasUnOp A) : Prop :=
   r_inv : forall x : A, x + - x == 0.
-
-Section Context.
-
-Context {A : Type} `{is_r_inv : IsRInv A}.
-
-Global Instance bin_op_un_un_op_is_r_ext_inv : IsRExtInv bin_op un un_op.
-Proof. intros x. apply r_inv. Qed.
-
-End Context.
