bird/Is/OneSortedly/UnaryAntidistributive.v
@@ -1,20 +1,8 @@
 From Maniunfold.Has Require Export
   EquivalenceRelation BinaryOperation UnaryOperation.
-From Maniunfold.Is Require Export
-  ExternallyUnaryAntidistributive.
 From Maniunfold.ShouldHave Require Import
   EquivalenceRelationNotations AdditiveNotations.
 
 Class IsUnaryAntidistr {A : Type} {has_eq_rel : HasEqRel A}
   (has_bin_op : HasBinOp A) (has_un_op : HasUnOp A) : Prop :=
   un_antidistr : forall x y : A, - (x + y) == - y + - x.
-
-Section Context.
-
-Context {A : Type} `{is_un_antidistr : IsUnaryAntidistr A}.
-
-Global Instance bin_op_un_op_is_ext_un_antidistr :
-  IsExtUnaryAntidistr bin_op un_op.
-Proof. intros x y. apply un_antidistr. Qed.
-
-End Context.
