bird/Is/ThreeSortedly/Bicompatible.v
@@ -1,0 +1,8 @@
+From Maniunfold.Has Require Export
+  OneSorted.EquivalenceRelation LeftAction RightAction.
+From Maniunfold.ShouldHave Require Import
+  EquivalenceRelationNotations AdditiveNotations.
+
+Class IsBicompat {A B C : Type} {has_eq_rel : HasEqRel C}
+  (has_l_act : HasLAct A C) (has_r_act : HasRAct B C) : Prop :=
+  bicompat : forall (x : A) (y : C) (z : B), x L+ (y R+ z) == (x L+ y) R+ z.
