bird/Is/TwoSortedly/LeftExternallyBinaryCommutative.v
@@ -1,8 +1,8 @@
 From Maniunfold.Has Require Export
-  OneSorted.BinaryRelation RightAction LeftUnaryOperation.
+  OneSorted.EquivalenceRelation RightAction LeftUnaryOperation.
 From Maniunfold.ShouldHave Require Import
-  BinaryRelationNotations AdditiveNotations.
+  EquivalenceRelationNotations AdditiveNotations.
 
-Class IsLExtBinComm {A B : Type} {has_bin_rel : HasBinRel B}
+Class IsLExtBinComm {A B : Type} {has_eq_rel : HasEqRel B}
   (has_l_un_op : HasLUnOp B) (has_r_act : HasRAct A B) : Prop :=
-  l_ext_bin_comm : forall (x : B) (y : A), L- (x R+ y) ~~ L- x R+ y.
+  l_ext_bin_comm : forall (x : B) (y : A), L- (x R+ y) == L- x R+ y.
