bird/Is/TwoSortedly/LeftInternallyInvertible.v
@@ -1,9 +1,0 @@
-From Maniunfold.Has Require Export
-  OneSorted.BinaryRelation BinaryFunction Unit Function.
-From Maniunfold.ShouldHave Require Import
-  BinaryRelationNotations AdditiveNotations.
-
-Class IsLIntInv {A B C : Type} {has_bin_rel : HasBinRel C}
-  (has_bin_fn : HasBinFn A B C) (has_un : HasUn C)
-  (has_fn : HasFn B A) : Prop :=
-  l_int_inv : forall x : B, T- x T+ x ~~ T0.
