bird/Is/TwoSortedly/RightCompatible.v
@@ -5,4 +5,4 @@ From Maniunfold.ShouldHave Require Import
 
 Class IsRCompat {A B : Type} {has_eq_rel : HasEqRel B}
   (has_bin_op : HasBinOp A) (has_r_act : HasRAct A B) : Prop :=
-  r_compat : forall (a b : A) (x : B), (x R+ a) R+ b == x R+ (a + b).
+  r_compat : forall (a b : A) (x : B), x R+ (a + b) == (x R+ a) R+ b.
