bird/Is/TwoSortedly/RightExternallyBinaryCommutative.v
@@ -1,8 +1,8 @@
 From Maniunfold.Has Require Export
-  OneSorted.BinaryRelation LeftAction RightUnaryOperation.
+  OneSorted.EquivalenceRelation LeftAction RightUnaryOperation.
 From Maniunfold.ShouldHave Require Import
-  BinaryRelationNotations AdditiveNotations.
+  EquivalenceRelationNotations AdditiveNotations.
 
-Class IsRExtBinComm {A B : Type} {has_bin_rel : HasBinRel B}
+Class IsRExtBinComm {A B : Type} {has_eq_rel : HasEqRel B}
   (has_r_un_op : HasRUnOp B) (has_l_act : HasLAct A B) : Prop :=
-  r_ext_bin_comm : forall (x : A) (y : B), R- (x L+ y) ~~ x L+ R- y.
+  r_ext_bin_comm : forall (x : A) (y : B), R- (x L+ y) == x L+ R- y.
