bird/Is/TwoSortedly/RightInternallyInvertible.v
@@ -1,9 +1,0 @@
-From Maniunfold.Has Require Export
-  OneSorted.BinaryRelation BinaryFunction Unit Function.
-From Maniunfold.ShouldHave Require Import
-  BinaryRelationNotations AdditiveNotations.
-
-Class IsRIntInv {A B C : Type} {has_bin_rel : HasBinRel C}
-  (has_bin_fn : HasBinFn B A C) (has_un : HasUn C)
-  (has_fn : HasFn B A) : Prop :=
-  r_int_inv : forall x : B, x T+ T- x ~~ T0.
